src/lowparse/LowParse.SLow.fst
@@ -1,14 +1,3 @@
 module LowParse.SLow
-include LowParse.SLow.Base
-include LowParse.SLow.Combinators
-include LowParse.SLow.Int
-include LowParse.SLow.List
-include LowParse.SLow.FLData
-include LowParse.SLow.VLData
-include LowParse.SLow.Array
-include LowParse.SLow.Bytes
-include LowParse.SLow.Enum
-include LowParse.SLow.Tac.Enum
-include LowParse.SLow.Sum
-include LowParse.SLow.Tac.Sum
-include LowParse.SLow.Option
+friend LowParse.SLow.Int
+friend LowParse.SLow.Array
