src/lowparse/LowParse.SLow.fsti
@@ -1,0 +1,14 @@
+module LowParse.SLow
+include LowParse.SLow.Base
+include LowParse.SLow.Combinators
+include LowParse.SLow.Int
+include LowParse.SLow.List
+include LowParse.SLow.FLData
+include LowParse.SLow.VLData
+include LowParse.SLow.Array
+include LowParse.SLow.Bytes
+include LowParse.SLow.Enum
+include LowParse.SLow.Tac.Enum
+include LowParse.SLow.Sum
+include LowParse.SLow.Tac.Sum
+include LowParse.SLow.Option
